$$\sum_{i=0}^n i^2 = \frac{(n^2+n)(2n+1)}{6}$$

$$(\frac{\sqrt x}{y^3})$$

$$\left(\frac{\sqrt x}{y^3}\right)$$

$$\sum_{i=0}^\infty \sqrt[3]{\frac iy}$$

$$
        \begin{matrix}
        1 & x & x^2 \\
        1 & y & y^2 \\
        1 & z & z^2 \\
        \end{matrix}
$$

$$ \left[
    \begin{array}{cc|c}
      1&2&3\\
      4&5&6
    \end{array}
\right] $$

$$
\begin{aligned}
\sqrt{37} & = \sqrt{\frac{73^2-1}{12^2}} \\
 & = \sqrt{\frac{73^2}{12^2}\cdot\frac{73^2-1}{73^2}} \\ 
 & = \sqrt{\frac{73^2}{12^2}}\sqrt{\frac{73^2-1}{73^2}} \\
 & = \frac{73}{12}\sqrt{1 - \frac{1}{73^2}} \\ 
 & \approx \frac{73}{12}\left(1 - \frac{1}{2\cdot73^2}\right)
\end{aligned}
$$

$$
\begin{array}{c|lcr} \\
1 & 0.24 & 1 & 125 \\
2 & -1 & 189 & -8 \\
3 & -20 & 2000 & 1+10i
\end{array}
$$

$$
\left\{ 
\begin{array}{c}
a_1x+b_1y+c_1z=d_1 \\ 
a_2x+b_2y+c_2z=d_2 \\ 
a_3x+b_3y+c_3z=d_3
\end{array}
\right. 
$$

$$\begin{cases}
a_1x+b_1y+c_1z=d_1 \\ 
a_2x+b_2y+c_2z=d_2 \\ 
a_3x+b_3y+c_3z=d_3
\end{cases}
$$

$$
\left\{
\begin{aligned} 
a_1x+b_1y+c_1z &=d_1+e_1 \\ 
a_2x+b_2y&=d_2 \\ 
a_3x+b_3y+c_3z &=d_3 
\end{aligned} 
\right. 
$$



